---
layout: post
title:  "My first post"
date:   2020-04-11 21:03:01 -0500
categories: jekyll update
published: true
---

$$L(w) = -\log p(t|w) = -\sum_{n=1}^{N}t_n\log y_n + (1-t_n)\log (1-y_n) $$
where $$y_n = \sigma(a)$$, $$a_n = w^T\phi_n $$
$$\frac{\partial L}{\partial w} = -\sum_{n=1}^{N}\partial_w (t_n\log y_n) + \partial_w (1-t_n)\log (1-y_n) $$
$$
\partial_w (t_n\log y_n) = \frac{\partial t_n\log y_n}{\partial \log y_n}
\frac{\partial \log y_n}{\partial y_n} \frac{\partial y_n}{\partial \sigma}
\frac{\partial \sigma}{\partial a} \frac{\partial a}{\partial w}  
= t_n * \frac{1}{y_n} * \sigma(1-\sigma) * \phi_n
$$
$$
\frac{\partial (1-t_n)\log (1-y_n)}{\partial \log (1-y_n)} 
\frac{\partial \log (1-y_n)}{y_n}
= (1-t_n)*\frac{1}{y_n-1}
$$
$$
\begin{align*}
\partial_w (t_n\log y_n) + \partial_w (1-t_n)\log (1-y_n) &= (-\frac{t_n}{y_n} + \frac{1-t_n}{1-y_n}) * \sigma(1-\sigma) * \phi_n \\
&= \frac{y_n-t_n}{y_n(1-y_n)} * \sigma(1-\sigma) * \phi_n
\end{align*}
$$
$$\frac{\partial L}{\partial w} = -\sum_{n=1}^{N}(y_n-t_n)*\phi_n $$